CppFormalization/Cpp2/Closure/Internal/All.lean
@@ -31,8 +31,8 @@ import CppFormalization.Cpp2.Closure.Internal.HeadTailReturnAwareCallbacksCI
 import CppFormalization.Cpp2.Closure.Internal.InternalClosureRoadmap
 import CppFormalization.Cpp2.Closure.Internal.InternalClosureRoadmapCI
 import CppFormalization.Cpp2.Closure.Internal.InternalClosureRoadmapConcrete
-import CppFormalization.Cpp2.Closure.Internal.LoopBodyDynamicReplayStateTheoremsCI
 import CppFormalization.Cpp2.Closure.Internal.LoopBodyDynamicReplayContinueStateTheoremsCI
+import CppFormalization.Cpp2.Closure.Internal.LoopBodyDynamicReplayStateTheoremsCI
 import CppFormalization.Cpp2.Closure.Internal.LoopBodyFunctionClosureCI
 import CppFormalization.Cpp2.Closure.Internal.LoopReentryKernelCI
 import CppFormalization.Cpp2.Closure.Internal.LoopReentryKernelSplitCI
@@ -40,7 +40,6 @@ import CppFormalization.Cpp2.Closure.Internal.NormalPathTypingBridge
 import CppFormalization.Cpp2.Closure.Internal.PrimitiveStmtNormalPreservation
 import CppFormalization.Cpp2.Closure.Internal.PtrExprAssignTransportKernel
 import CppFormalization.Cpp2.Closure.Internal.ReadinessBoundaryConcrete
-import CppFormalization.Cpp2.Closure.Internal.LoopBodyDynamicReplayStateTheoremsCI
 import CppFormalization.Cpp2.Closure.Internal.ReadinessReplayPrimitive
 import CppFormalization.Cpp2.Closure.Internal.ReadinessResidualBoundary
 import CppFormalization.Cpp2.Closure.Internal.ReadinessTransportNormal
